Finish refactor

src/verification/semantics/skip_stream_multiply.lean
@@ -25,6 +25,10 @@ subrelation.wf rprod_eq_sub_lex (lex_wf h₁ h₂)
 
 end prod
 
+lemma mul_eq_zero_of {α : Type*} [mul_zero_class α] {x y : α} : x = 0 ∨ y = 0 → x * y = 0
+| (or.inl h) := by { rw h, exact zero_mul y, }
+| (or.inr h) := by { rw h, exact mul_zero x, }
+
 open_locale streams
 variables {ι : Type} [linear_order ι] {α : Type*}
 
@@ -41,7 +45,7 @@ def Stream.mul [has_mul α] (a b : Stream ι α) : Stream ι α :=
 { σ := a.σ × b.σ,
   valid := λ p, a.valid p.1 ∧ b.valid p.2,
   ready := λ p, Stream.mul.ready a b p,
-  skip := λ p hp i r, (a.skip p.1 hp.1 i r, b.skip p.2 hp.2 i r),
+  skip := λ p hp i, (a.skip p.1 hp.1 i, b.skip p.2 hp.2 i),
   index := λ p hv, max (a.index p.1 hv.1) (b.index p.2 hv.2),
   value := λ p hr, a.value p.1 hr.r₁ * b.value p.2 hr.r₂ }
 
@@ -53,8 +57,8 @@ lemma Stream.mul.ready.index' {a : Stream ι α} {b : Stream ι α} {x y} (h : (
 by simp [Stream.index'_val h.v₁, Stream.index'_val h.v₂, h.index]
 
 lemma Stream.mul.ready.order_eq {a : Stream ι α} {b : Stream ι α} {x y} (h : (a.mul b).ready (x, y)) :
-  a.to_order x = b.to_order y :=
-by ext : 1; simp [h.r₁, h.r₂, h.index']
+  a.to_order x h.v₁ = b.to_order y h.v₂ :=
+by { dsimp only [Stream.to_order], simp [h.r₁, h.r₂, h.index], }
 
 lemma Stream.mul_index' (a b : Stream ι α) (xy : a.σ × b.σ) :
   (a.mul b).index' xy = max (a.index' xy.1) (b.index' xy.2) :=
@@ -68,18 +72,18 @@ begin
 end
 
 lemma order_eq_of_mul_ready {a b : Stream ι α} {x y} (h : (a.mul b).ready (x, y)) :
-  a.to_order x = (a.mul b).to_order (x, y) ∧ b.to_order y = (a.mul b).to_order (x, y) :=
-by { split; simp only [Stream.to_order, h, h.r₁, h.r₂]; simp [Stream.mul_index', Stream.mul.ready.index' h], } 
+  a.to_order x h.v₁ = (a.mul b).to_order (x, y) ⟨h.v₁, h.v₂⟩ ∧ b.to_order y h.v₂ = (a.mul b).to_order (x, y) ⟨h.v₁, h.v₂⟩ :=
+by { split; simp only [Stream.to_order, h, h.r₁, h.r₂]; simp [h.index], } 
 
 /-- This lemma takes a surprising amount of effort to prove -/
 lemma min_to_order_le (a b : Stream ι α) (q : a.σ × b.σ) (hv : (a.mul b).valid q) :
-  min (a.to_order q.1) (b.to_order q.2) ≤ (a.mul b).to_order q :=
+  min (a.to_order q.1 hv.1) (b.to_order q.2 hv.2) ≤ (a.mul b).to_order q hv :=
 begin
   rw prod.lex.le_iff'', 
-  simp only [monotone.map_min (@prod.lex.fst_mono (with_top ι) bool _ _)],
-  split, { convert min_le_max, simp [Stream.mul_index'], },
+  simp only [monotone.map_min (@prod.lex.fst_mono ι bool _ _)],
+  split, { exact min_le_max, },
   intro h,
-  replace h : a.index' q.1 = b.index' q.2 := by simpa [Stream.mul_index'] using h,
+  simp only [Stream.to_order_fst, Stream.mul_index, max_eq_min_iff] at h,
   suffices : a.ready q.1 → b.ready q.2 → (a.mul b).ready q,
   { simpa [Stream.to_order, h, prod.lex.mk_min, bool.min_eq_and, bool.le_iff_imp], },
   intros hr₁ hr₂,
@@ -88,38 +92,33 @@ begin
 end
 
 lemma to_order_le_max (a b : Stream ι α) (q : a.σ × b.σ) (hv : (a.mul b).valid q) :
-  (a.mul b).to_order q ≤ max (a.to_order q.1) (b.to_order q.2) :=
+  (a.mul b).to_order q hv ≤ max (a.to_order q.1 hv.1) (b.to_order q.2 hv.2) :=
 begin
   rw prod.lex.le_iff', right, split,
-  { simp [monotone.map_max (@prod.lex.fst_mono (with_top ι) bool _ _), Stream.mul_index'], },
+  { simp [monotone.map_max (@prod.lex.fst_mono ι bool _ _), Stream.mul_index'], },
   simp only [bool.le_iff_imp, Stream.to_order_snd, bool.of_to_bool_iff],
   intro hr, cases q with qa qb,
   simpa [order_eq_of_mul_ready hr],
 end
 
-def BoundedStream.mul (a b : BoundedStream ι α) : BoundedStream ι α :=
-{ wf_rel := prod.rprod_eq a.wf_rel b.wf_rel,
-  wf := prod.rprod_eq_wf a.wf b.wf,
-  wf_valid := λ q hq i r, begin
-    rcases a.wf_valid q.1 hq.1 i r with (h|⟨ha₁, ha₂⟩),
-    { exact or.inl (or.inl ⟨h, b.no_backward _ _ _ _⟩), },
-    rcases b.wf_valid q.2 hq.2 i r with (h|⟨hb₁, hb₂⟩),
-    { exact or.inl (or.inr ⟨h, a.no_backward _ _ _ _⟩), },
-    right, split, swap,
-    { dsimp, simp [ha₂, hb₂], },
-    exact lt_of_lt_of_le (lt_min ha₁ hb₁) (min_to_order_le _ _ _ hq),
-  end ,
-  ..(a.mul b.to_Stream) }
-
-@[simp] lemma BoundedStream.mul_to_Stream (a b : BoundedStream ι α) :
-  (a.mul b).to_Stream = a.to_Stream.mul b.to_Stream := rfl
+instance Stream.mul.is_bounded (a b : Stream ι α) [is_bounded a] [is_bounded b] : is_bounded (a.mul b) :=
+⟨⟨prod.rprod_eq a.wf_rel b.wf_rel, prod.rprod_eq_wf a.wf b.wf,
+λ q hq i, begin
+  rcases a.wf_valid q.1 hq.1 i with (h|⟨ha₁, ha₂⟩),
+  { exact or.inl (or.inl ⟨h, b.no_backward _ _ _⟩), },
+  rcases b.wf_valid q.2 hq.2 i with (h|⟨hb₁, hb₂⟩),
+  { exact or.inl (or.inr ⟨h, a.no_backward _ _ _⟩), },
+  right, split, swap,
+  { dsimp, simp [ha₂, hb₂], },
+  exact lt_of_lt_of_le (lt_min ha₁ hb₁) (min_to_order_le _ _ _ hq),
+end⟩⟩
 
 end index_lemmas
 
 section value_lemmas
 variables [non_unital_non_assoc_semiring α]
 
-lemma mul_eval₀_of_neq {a : Stream ι α} {b : Stream ι α} {x y} (h : a.to_order x ≠ b.to_order y) (H) :
+lemma mul_eval₀_of_neq {a : Stream ι α} {b : Stream ι α} {x y} (H : (a.mul b).valid (x, y)) (h : a.to_order x H.1 ≠ b.to_order y H.2) :
   (a.mul b).eval₀ (x, y) H = 0 :=
 by { contrapose! h, apply Stream.mul.ready.order_eq, simp [Stream.eval₀] at h, exact h.fst, }
 
@@ -133,92 +132,87 @@ begin
   rw finsupp.mul_single_eq_zero _ _ (hr h₁ h₂),
 end
 
-lemma mul_eval₀_spec (a b : BoundedStream ι α)
-  (ha : a.is_strict_mono) (hb : b.is_strict_mono) (q : (a.mul b).σ) (hv : Stream.valid _ q) :
-  (a.mul b).eval₀ q hv = ((a.eval q.1) * (b.eval q.2)).filter (λ i, (↑i, ff) <ₗ (a.mul b).to_order q) :=
+lemma mul_eval₀_spec (a b : Stream ι α) [is_bounded a] [is_bounded b]
+  (ha : a.is_strict_mono) (hb : b.is_strict_mono) (q : (a.mul b).σ) (hv : (a.mul b).valid q) :
+  (a.mul b).eval₀ q hv = ((a.eval q.1) * (b.eval q.2)).filter (λ i, (i, ff) <ₗ (a.mul b).to_order q hv) :=
 begin
   classical,
   by_cases H : (a.mul b).ready q,
   { cases q with qa qb,
     calc (a.mul b).eval₀ (qa, qb) hv 
         = (a.eval₀ qa hv.1) * (b.eval₀ qb hv.2) : by { dsimp, rw [mul_eval₀], }
-    ... = (a.eval qa).filter (λ i, (↑i, ff) <ₗ a.to_order qa) *
-            (b.eval qb).filter (λ i, (↑i, ff) <ₗ b.to_order qb) : by rw [ha.eval₀_eq_eval_filter, hb.eval₀_eq_eval_filter]
-    ... = ((a.eval qa) * (b.eval qb)).filter (λ i, (↑i, ff) <ₗ min (a.to_order qa) (b.to_order qb)) : by simp only [finsupp.mul_filter, lt_min_iff]
-    ... = ((a.eval qa) * (b.eval qb)).filter (λ i, (↑i, ff) <ₗ (a.mul b).to_order (qa, qb)) : 
+    ... = (a.eval qa).filter (λ i, (i, ff) <ₗ a.to_order qa hv.1) *
+            (b.eval qb).filter (λ i, (i, ff) <ₗ b.to_order qb hv.2) : by rw [ha.eval₀_eq_eval_filter, hb.eval₀_eq_eval_filter]
+    ... = ((a.eval qa) * (b.eval qb)).filter (λ i, (i, ff) <ₗ min (a.to_order qa hv.1) (b.to_order qb hv.2)) : by simp only [finsupp.mul_filter, lt_min_iff]
+    ... = ((a.eval qa) * (b.eval qb)).filter (λ i, (i, ff) <ₗ (a.mul b).to_order (qa, qb) hv) : 
             by { congr, ext i, simp [(order_eq_of_mul_ready H).1, (order_eq_of_mul_ready H).2], refl, } },
   { symmetry,
-    simp only [Stream.eval₀, H, dif_neg, not_false_iff, finsupp.filter_eq_zero_iff, Stream.to_order], dsimp only [BoundedStream.mul_to_Stream],
-    simp only [to_bool_false_eq_ff, prod.lex.mk_snd_mono_lt_iff, finsupp.mul_apply, Stream.mul_index', lt_max_iff],
-    intros i hi, cases hi.imp (ha.1.eq_zero_of_lt_index i) (hb.1.eq_zero_of_lt_index i) with h h; simp [h], }
+    simp only [Stream.eval₀, H, dif_neg, not_false_iff, finsupp.filter_eq_zero_iff, Stream.to_order,
+      to_bool_false_eq_ff, prod.lex.mk_snd_mono_lt_iff, finsupp.mul_apply, Stream.mul_index, lt_max_iff],
+    intros i hi, 
+    refine mul_eq_zero_of (hi.imp (λ h, ha.1.eq_zero_of_lt_index i _) (λ h, hb.1.eq_zero_of_lt_index i _));
+    simpa [hv.1, hv.2] using h, }
 end
 
 lemma mul_mono {a b : Stream ι α} (ha : a.is_monotonic) (hb : b.is_monotonic) :
   (a.mul b).is_monotonic :=
-by { intros q hv i r, simp only [Stream.mul_index'], exact max_le_max (ha _ _ _ _) (hb _ _ _ _), }
+by { intros q hv i, simp only [Stream.mul_index'], exact max_le_max (ha _ _ _) (hb _ _ _), }
 
 lemma mul_strict_mono {a b : Stream ι α} (ha : a.is_strict_mono) (hb : b.is_strict_mono) :
   (a.mul b).is_strict_mono :=
-⟨mul_mono ha.1 hb.1, λ q hv i r H hr, ne_of_lt begin
+⟨mul_mono ha.1 hb.1, λ q hv i H hr, ne_of_lt begin
   simp only [Stream.mul_index'],
   cases q with qa qb,
-  refine max_lt_max (ha.lt _ _ _ _ _ hr.r₁) (hb.lt _ _ _ _ _ hr.r₂);
+  refine max_lt_max (ha.lt _ _ _ _ hr.r₁) (hb.lt _ _ _ _ hr.r₂);
   simpa [order_eq_of_mul_ready hr],
 end⟩
 
-local notation ` ↑ₛ `:1000 a := a.to_BoundedStream
-
-lemma next_eval_mul_eq (a b : StrictLawfulStream ι α) (q : ((↑ₛa).mul (↑ₛb)).σ) (hv : Stream.valid _ q) :
-  (a.eval $ (((↑ₛa).mul (↑ₛb)).next q).1) * (b.eval $ (((↑ₛa).mul (↑ₛb)).next q).2) =
-    ((a.eval q.1) * (b.eval q.2)).filter (λ i, ((↑ₛa).mul (↑ₛb)).to_order q ≤ (↑i, ff)) :=
+lemma next_eval_mul_eq (a b : Stream ι α) [is_strict_lawful a] [is_strict_lawful b] (q : (a.mul b).σ) (hv : (a.mul b).valid q) :
+  (a.eval ((a.mul b).next q).1) * (b.eval ((a.mul b).next q).2) =
+    ((a.eval q.1) * (b.eval q.2)).filter (λ i, (a.mul b).to_order q hv ≤ (i, ff)) :=
 begin
   ext j,
   simp only [finsupp.mul_apply, finsupp.filter_apply, Stream.next_val hv],
   split_ifs with hj,
-  { simp only [Stream.to_order, Stream.index'_val hv] at hj,
-    dsimp only [BoundedStream.mul_to_Stream, Stream.mul_skip] at hj ⊢,
-    rw [a.skip_spec q.1 hv.1 _ _ _ hj, b.skip_spec q.2 hv.2 _ _ _ hj], },
-  change (a.eval (a.skip _ _ _ _) j) * (b.eval (b.skip _ _ _ _) j) = 0,
+  { simp only [Stream.to_order, Stream.index'_val hv, Stream.mul_skip] at hj ⊢,
+    rw [is_lawful.skip_spec q.1 hv.1 _ _ hj, is_lawful.skip_spec q.2 hv.2 _ _ hj], },
+  change (a.eval (a.skip _ _ _) j) * (b.eval (b.skip _ _ _) j) = 0,
   rw not_le at hj,
   cases (le_max_iff.mp $ to_order_le_max _ _ _ hv) with hj' hj',
-  { rw [a.strict_mono.eval_skip_eq_zero, zero_mul],
-    { convert hj, rw [Stream.index'_val hv], }, { convert hj', rw ← Stream.index'_val, refl, }, },
-  { rw [b.strict_mono.eval_skip_eq_zero, mul_zero],
-    { convert hj, rw [Stream.index'_val hv], }, { convert hj', rw ← Stream.index'_val, refl, }, },
-  
+  { rw [a.strict_mono.eval_skip_eq_zero, zero_mul]; assumption, },
+  { rw [b.strict_mono.eval_skip_eq_zero, mul_zero]; assumption, },
 end
 
-lemma mul_spec (a b : StrictLawfulStream ι α) (q : ((↑ₛa).mul (↑ₛb)).σ) :
-  (BoundedStream.eval _ q) = (a.eval q.1) * (b.eval q.2) :=
+lemma mul_spec (a b : Stream ι α) [is_strict_lawful a] [is_strict_lawful b] (q : (a.mul b).σ) :
+  ((a.mul b).eval q) = (a.eval q.1) * (b.eval q.2) :=
 begin
-  refine @well_founded.induction _ (a.to_BoundedStream.mul b.to_BoundedStream).wf_rel (a.to_BoundedStream.mul b.to_BoundedStream).wf _ q _,
+  refine @well_founded.induction _ (a.mul b).wf_rel (a.mul b).wf _ q _,
   clear q, intros q ih,
-  by_cases hv : ((↑ₛa).mul (↑ₛb)).valid q, swap,
+  by_cases hv : (a.mul b).valid q, swap,
   { cases not_and_distrib.mp hv with hv' hv'; simp [hv, hv'], },
-  rw [BoundedStream.eval_valid _ _ hv, ih _ (((↑ₛa).mul (↑ₛb)).next_wf q hv),
+  rw [Stream.eval_valid _ _ hv, ih _ ((a.mul b).next_wf q hv),
     next_eval_mul_eq _ _ _ hv, mul_eval₀_spec _ _ a.strict_mono b.strict_mono _ hv],
   convert finsupp.filter_pos_add_filter_neg _ _,
   simp,
 end
 
-lemma mul_skip_spec (a b : StrictLawfulStream ι α) (q : ((↑ₛa).mul (↑ₛb)).σ) (hq : Stream.valid _ q)
-  (i : ι) (r : bool) (j : ι) (h : ((↑i : with_top ι), r) ≤ₗ (↑j, ff)) :
-  ((↑ₛa).mul (↑ₛb)).eval (((↑ₛa).mul (↑ₛb)).skip q hq i r) j = ((↑ₛa).mul (↑ₛb)).eval q j :=
+lemma mul_skip_spec (a b : Stream ι α) [is_strict_lawful a] [is_strict_lawful b] (q : (a.mul b).σ) (hq : (a.mul b).valid q)
+  (i : ι ×ₗ bool) (j : ι) (h : i ≤ₗ (j, ff)) :
+  (a.mul b).eval ((a.mul b).skip q hq i) j = (a.mul b).eval q j :=
 begin
   simp only [finsupp.mul_apply, mul_spec], congr' 1;
-  { dsimp, rw LawfulStream.skip_spec, assumption, }
+  { dsimp, rwa is_lawful.skip_spec, }
 end
 
-def StrictLawfulStream.mul (a b : StrictLawfulStream ι α) : StrictLawfulStream ι α :=
+instance Stream.mul.is_strict_lawful (a b : Stream ι α) [is_strict_lawful a] [is_strict_lawful b] : is_strict_lawful (a.mul b) :=
 { skip_spec := mul_skip_spec a b,
   mono := (mul_strict_mono a.strict_mono b.strict_mono).1,
-  strict_mono := mul_strict_mono a.strict_mono b.strict_mono,
-  ..(a.to_BoundedStream.mul b.to_BoundedStream) }
+  strict_mono := mul_strict_mono a.strict_mono b.strict_mono, }
 
-instance : has_mul (StrictLawfulStream ι α) := ⟨StrictLawfulStream.mul⟩
+instance : has_mul (Stream ι α) := ⟨Stream.mul⟩
 
-@[simp] lemma StrictLawfulStream.mul_spec (a b : StrictLawfulStream ι α) (q : (a * b).σ) :
+@[simp] lemma StrictLawfulStream.mul_spec (a b : Stream ι α) [is_strict_lawful a] [is_strict_lawful b] (q : (a * b).σ) :
   (a * b).eval q = (a.eval q.1) * (b.eval q.2) :=
-by { change (a.to_BoundedStream.mul b.to_BoundedStream).eval q = _, rw mul_spec, }
+by { change (a.mul b).eval q = _, rw mul_spec, }
 
 end value_lemmas
